src/tls/Negotiation.Writers.fst
@@ -23,101 +23,38 @@ open Negotiation
 
 (* implementation of the new spec *)
 
-let write_binder_ph
+module LPW = LowParse.Low.Writers
+
+assume val write_binder_ph
   (#rrel #rel: _)
   (sin: LP.slice rrel rel)
   (pin: U32.t)
+  (h0: HS.mem)
   (sout: LP.slice (LP.srel_of_buffer_srel (B.trivial_preorder _)) (LP.srel_of_buffer_srel (B.trivial_preorder _)))
-  (pout_from: U32.t)
-: HST.Stack U32.t
-  (requires (fun h ->
-    LP.live_slice h sin /\
-    LP.live_slice h sout /\
-    U32.v pout_from <= U32.v sout.LP.len /\
-    U32.v sout.LP.len < U32.v LP.max_uint32 /\ // to error code
-    LP.valid Parsers.TicketContents13.ticketContents13_parser h sin pin /\
-    B.loc_disjoint (LP.loc_slice_from_to sin pin (LP.get_valid_pos Parsers.TicketContents13.ticketContents13_parser h sin pin)) (LP.loc_slice_from sout pout_from)
-  ))
-  (ensures (fun h pout_to h' ->
-    B.modifies (LP.loc_slice_from sout pout_from) h h' /\ (
-    let ph = compute_binder_ph_new (LP.contents Parsers.TicketContents13.ticketContents13_parser h sin pin) in
-    if pout_to = LP.max_uint32
-    then
-      U32.v pout_from + LP.serialized_length pskBinderEntry_serializer ph > U32.v sout.LP.len
-    else
-      LP.valid_content_pos pskBinderEntry_parser h' sout pout_from ph pout_to
-  )))
-= let h0 = HST.get () in
-  let ph = Ghost.hide (compute_binder_ph_new (LP.contents Parsers.TicketContents13.ticketContents13_parser h0 sin pin)) in
-  let c = CipherSuite.cipherSuite13_reader sin (Parsers.TicketContents13.accessor_ticketContents13_cs sin pin) in
-  let (CipherSuite13 _ h) = cipherSuite_of_cipherSuite13 c in
-  let len : U32.t = Hashing.Spec.tagLen h in
-  if (1ul `U32.add` len) `U32.gt` (sout.LP.len `U32.sub` pout_from)
-  then begin
-    LP.serialized_length_eq pskBinderEntry_serializer (Ghost.reveal ph);
-    pskBinderEntry_bytesize_eq (Ghost.reveal ph);
-    LP.max_uint32
-  end else begin
-    let pout_payload = pout_from `U32.add` 1ul in
-    // TODO: replace with a custom fill once target slice is replaced with the stash
-    B.fill (B.sub sout.LP.base pout_payload len) 0uy len;
-    pskBinderEntry_finalize sout pout_from len
-  end
+  (pout_from: U32.t {
+    LP.valid Parsers.TicketContents13.ticketContents13_parser h0 sin pin /\
+    B.loc_disjoint (LP.loc_slice_from_to sin pin (LP.get_valid_pos Parsers.TicketContents13.ticketContents13_parser h0 sin pin)) (LP.loc_slice_from sout pout_from)
+  })
+: Tot (w: LPW.writer pskBinderEntry_serializer h0 sout pout_from {
+  LPW.wvalue w == compute_binder_ph_new (LP.contents Parsers.TicketContents13.ticketContents13_parser h0 sin pin)
+})
 
-
-#push-options "--z3rlimit 32"
-
-let write_obfuscate_age
+assume val write_obfuscate_age
   (now: U32.t)
   (#rrel #rel: _)
   (sin: LP.slice rrel rel)
   (pin: U32.t)
+  (h0: HS.mem)
   (sout: LP.slice (LP.srel_of_buffer_srel (B.trivial_preorder _)) (LP.srel_of_buffer_srel (B.trivial_preorder _)))
-  (pout_from: U32.t)
-: HST.Stack U32.t
-  (requires (fun h ->
-    LP.valid Parsers.ResumeInfo13.resumeInfo13_parser h sin pin /\
-    B.loc_disjoint (LP.loc_slice_from_to sin pin (LP.get_valid_pos Parsers.ResumeInfo13.resumeInfo13_parser h sin pin)) (LP.loc_slice_from sout pout_from) /\
-    LP.live_slice h sout /\
-    U32.v pout_from <= U32.v sout.LP.len /\
-    U32.v sout.LP.len < U32.v LP.max_uint32
-  ))
-  (ensures (fun h res h' ->
-    let x = obfuscate_age_new now (LP.contents Parsers.ResumeInfo13.resumeInfo13_parser h sin pin) in
-    B.modifies (LP.loc_slice_from sout pout_from) h h' /\ (
-    if res = LP.max_uint32
-    then U32.v pout_from + LP.serialized_length pskIdentity_serializer x > U32.v sout.LP.len
-    else LP.valid_content_pos pskIdentity_parser h' sout pout_from x res
-  )))
-= let h = HST.get () in
-  let x = Ghost.hide (obfuscate_age_new now (LP.contents Parsers.ResumeInfo13.resumeInfo13_parser h sin pin)) in
-  LP.serialized_length_eq pskIdentity_serializer (Ghost.reveal x);
-  pskIdentity_bytesize_eq (Ghost.reveal x);
-  let sin_id = Parsers.ResumeInfo13.accessor_resumeInfo13_identity sin pin in
-  pskIdentity_identity_bytesize_eq ((Ghost.reveal x).identity);
-  LP.serialized_length_eq pskIdentity_identity_serializer ((Ghost.reveal x).identity);
-  let pout_oage = LP.copy_weak _ pskIdentity_identity_jumper sin sin_id sout pout_from in
-  if pout_oage = LP.max_uint32
-  then LP.max_uint32
-  else if 4ul `U32.gt` (sout.LP.len `U32.sub` pout_oage)
-  then LP.max_uint32
-  else begin
-    let pin_tkt = Parsers.ResumeInfo13.accessor_resumeInfo13_ticket sin pin in
-    let creation_time = LowParse.Low.Int.read_u32 sin (Parsers.TicketContents13.accessor_ticketContents13_creation_time sin pin_tkt) in
-    let age = FStar.UInt32.((now -%^ creation_time) *%^ 1000ul) in
-    let age_add = LowParse.Low.Int.read_u32 sin (Parsers.TicketContents13.accessor_ticketContents13_age_add sin pin_tkt) in
-    let obfuscated_age = PSK.encode_age age age_add in
-    let pout_to = LowParse.Low.Int.write_u32 obfuscated_age sout pout_oage in
-    let h' = HST.get () in
-    pskIdentity_valid h' sout pout_from;
-    pout_to
-  end
+  (pout_from: U32.t {
+    LP.valid Parsers.ResumeInfo13.resumeInfo13_parser h0 sin pin /\
+    B.loc_disjoint (LP.loc_slice_from_to sin pin (LP.get_valid_pos Parsers.ResumeInfo13.resumeInfo13_parser h0 sin pin)) (LP.loc_slice_from sout pout_from)
+  })
+: Tot (w: LPW.writer pskIdentity_serializer h0 sout pout_from { LPW.wvalue w == obfuscate_age_new now (LP.contents Parsers.ResumeInfo13.resumeInfo13_parser h0 sin pin) })
 
 #pop-options
 
 (* then, the writer *)
-
-module LPW = LowParse.Low.Writers
 
 let make_offeredPsks_identities
   (oidentities: option (list Parsers.PskIdentity.pskIdentity))
@@ -125,14 +62,12 @@ let make_offeredPsks_identities
 = match oidentities with
   | Some identities ->
     if
-      (let x = offeredPsks_identities_list_bytesize identities in 7 <= x && x <= 65535)
+      check_offeredPsks_identities_list_bytesize identities
     then Some identities
     else None
   | _ -> None
 
-inline_for_extraction
-noextract
-let write_offeredPsks_identities
+assume val write_offeredPsks_identities
   (#h0: HS.mem)
   (#sout: _)
   (#pout_from0: _)
@@ -140,44 +75,6 @@ let write_offeredPsks_identities
 : Tot (y: LPW.owriter Parsers.OfferedPsks_identities.offeredPsks_identities_serializer h0 sout pout_from0 {
     LPW.owvalue y == make_offeredPsks_identities (LPW.olwvalue w)
   })
-= LPW.OWriter (Ghost.hide (make_offeredPsks_identities (LPW.olwvalue w))) (fun pout_from ->
-    let f () : Lemma
-      (requires (Some? (make_offeredPsks_identities (LPW.olwvalue w))))
-      (ensures (
-        match make_offeredPsks_identities (LPW.olwvalue w) with
-        | None -> False
-        | Some oi ->
-          Some? (LPW.olwvalue w) /\
-          LP.serialized_length Parsers.OfferedPsks_identities.offeredPsks_identities_serializer oi == 2 + LP.serialized_list_length Parsers.PskIdentity.pskIdentity_serializer (Some?.v (LPW.olwvalue w))
-      ))
-    = match make_offeredPsks_identities (LPW.olwvalue w) with
-      | None -> ()
-      | Some oi ->
-        LP.serialized_length_eq Parsers.OfferedPsks_identities.offeredPsks_identities_serializer oi;
-        Parsers.OfferedPsks_identities.offeredPsks_identities_bytesize_eq oi;
-        Parsers.OfferedPsks_identities.offeredPsks_identities_list_bytesize_eq (Some?.v (LPW.olwvalue w))
-    in
-    assert (U32.v pout_from <= U32.v sout.LP.len);
-    Classical.move_requires f ();
-    if 2ul `U32.gt` (sout.LP.len `U32.sub` pout_from)
-    then LP.max_uint32
-    else
-      let res = LPW.olwrite w (pout_from `U32.add` 2ul) in
-      if (LP.max_uint32 `U32.sub` 1ul) `U32.lte` res
-      then
-        res
-      else begin
-        let h = HST.get () in
-        LP.valid_list_serialized_list_length Parsers.PskIdentity.pskIdentity_serializer h sout (pout_from `U32.add` 2ul) res;
-        let len = res `U32.sub` (pout_from `U32.add` 2ul) in
-        if len `U32.lt` 7ul || 65535ul `U32.lt` len
-        then LP.max_uint32 `U32.sub` 1ul
-        else begin
-          Parsers.OfferedPsks_identities.finalize_offeredPsks_identities sout pout_from res;
-          res
-        end
-      end
-  )
 
 let make_offeredPsks_binders
   (obinders: option (list Parsers.PskBinderEntry.pskBinderEntry))
@@ -185,16 +82,14 @@ let make_offeredPsks_binders
 = match obinders with
   | Some binders ->
     if
-      (let x = offeredPsks_binders_list_bytesize binders in 33 <= x && x <= 65535)
+      check_offeredPsks_binders_list_bytesize binders
     then begin
       Some binders
     end
     else None
   | _ -> None
 
-inline_for_extraction
-noextract
-let write_offeredPsks_binders
+assume val write_offeredPsks_binders
   (#h0: HS.mem)
   (#sout: _)
   (#pout_from0: _)
@@ -202,44 +97,6 @@ let write_offeredPsks_binders
 : Tot (y: LPW.owriter Parsers.OfferedPsks_binders.offeredPsks_binders_serializer h0 sout pout_from0 {
     LPW.owvalue y == make_offeredPsks_binders (LPW.olwvalue w)
   })
-= LPW.OWriter (Ghost.hide (make_offeredPsks_binders (LPW.olwvalue w))) (fun pout_from ->
-    let f () : Lemma
-      (requires (Some? (make_offeredPsks_binders (LPW.olwvalue w))))
-      (ensures (
-        match make_offeredPsks_binders (LPW.olwvalue w) with
-        | None -> False
-        | Some oi ->
-          Some? (LPW.olwvalue w) /\
-          LP.serialized_length Parsers.OfferedPsks_binders.offeredPsks_binders_serializer oi == 2 + LP.serialized_list_length Parsers.PskBinderEntry.pskBinderEntry_serializer (Some?.v (LPW.olwvalue w))
-      ))
-    = match make_offeredPsks_binders (LPW.olwvalue w) with
-      | None -> ()
-      | Some oi ->
-        LP.serialized_length_eq Parsers.OfferedPsks_binders.offeredPsks_binders_serializer oi;
-        Parsers.OfferedPsks_binders.offeredPsks_binders_bytesize_eq oi;
-        Parsers.OfferedPsks_binders.offeredPsks_binders_list_bytesize_eq (Some?.v (LPW.olwvalue w))
-    in
-    assert (U32.v pout_from <= U32.v sout.LP.len);
-    Classical.move_requires f ();
-    if 2ul `U32.gt` (sout.LP.len `U32.sub` pout_from)
-    then LP.max_uint32
-    else
-      let res = LPW.olwrite w (pout_from `U32.add` 2ul) in
-      if (LP.max_uint32 `U32.sub` 1ul) `U32.lte` res
-      then
-        res
-      else begin
-        let h = HST.get () in
-        LP.valid_list_serialized_list_length Parsers.PskBinderEntry.pskBinderEntry_serializer h sout (pout_from `U32.add` 2ul) res;
-        let len = res `U32.sub` (pout_from `U32.add` 2ul) in
-        if len `U32.lt` 33ul || 65535ul `U32.lt` len
-        then LP.max_uint32 `U32.sub` 1ul
-        else begin
-          Parsers.OfferedPsks_binders.finalize_offeredPsks_binders sout pout_from res;
-          res
-        end
-      end
-  )
 
 let make_preSharedKeyClientExtension
   (oi: option Parsers.OfferedPsks_identities.offeredPsks_identities)
@@ -251,9 +108,7 @@ let make_preSharedKeyClientExtension
 
 #push-options "--z3rlimit 16"
 
-inline_for_extraction
-noextract
-let write_preSharedKeyClientExtension
+assume val write_preSharedKeyClientExtension
   (#h0: _)
   (#sout: _)
   (#pout_from0: _)
@@ -262,44 +117,6 @@ let write_preSharedKeyClientExtension
 : Tot (y: LPW.owriter Parsers.PreSharedKeyClientExtension.preSharedKeyClientExtension_serializer h0 sout pout_from0 {
     LPW.owvalue y == make_preSharedKeyClientExtension (LPW.owvalue w_identities) (LPW.owvalue w_binders)
   })
-= LPW.OWriter (Ghost.hide (make_preSharedKeyClientExtension (LPW.owvalue w_identities) (LPW.owvalue w_binders))) (fun pout_from ->
-    Parsers.PreSharedKeyClientExtension.preSharedKeyClientExtension_parser_serializer_eq ();
-    let f () : Lemma
-      (requires (Some? (make_preSharedKeyClientExtension (LPW.owvalue w_identities) (LPW.owvalue w_binders))))
-      (ensures (
-        match make_preSharedKeyClientExtension (LPW.owvalue w_identities) (LPW.owvalue w_binders) with
-        | None -> False
-        | Some w ->
-          LP.serialized_length Parsers.PreSharedKeyClientExtension.preSharedKeyClientExtension_serializer w ==
-            LP.serialized_length Parsers.OfferedPsks_identities.offeredPsks_identities_serializer (Some?.v (LPW.owvalue w_identities)) +
-            LP.serialized_length Parsers.OfferedPsks_binders.offeredPsks_binders_serializer (Some?.v (LPW.owvalue w_binders))
-      ))
-    = match make_preSharedKeyClientExtension (LPW.owvalue w_identities) (LPW.owvalue w_binders) with
-      | None -> ()
-      | Some w ->
-        Parsers.OfferedPsks.offeredPsks_bytesize_eq w;
-        LP.serialized_length_eq Parsers.OfferedPsks.offeredPsks_serializer w;
-        Parsers.OfferedPsks_identities.offeredPsks_identities_bytesize_eq (Some?.v (LPW.owvalue w_identities));
-        LP.serialized_length_eq Parsers.OfferedPsks_identities.offeredPsks_identities_serializer (Some?.v (LPW.owvalue w_identities));
-        Parsers.OfferedPsks_binders.offeredPsks_binders_bytesize_eq (Some?.v (LPW.owvalue w_binders));
-        LP.serialized_length_eq Parsers.OfferedPsks_binders.offeredPsks_binders_serializer (Some?.v (LPW.owvalue w_binders))
-    in
-    Classical.move_requires f ();
-    let res1 = LPW.owrite w_identities pout_from in
-    if (LP.max_uint32 `U32.sub` 1ul) `U32.lte` res1
-    then res1
-    else begin
-      let res2 = LPW.owrite w_binders res1 in
-      if (LP.max_uint32 `U32.sub` 1ul) `U32.lte` res2
-      then
-        res2
-      else begin
-        let h = HST.get () in
-        Parsers.OfferedPsks.offeredPsks_valid h sout pout_from;
-        res2
-        end
-      end
-  )
 
 let make_clientHelloExtension_CHE_pre_shared_key
   (o: option Parsers.PreSharedKeyClientExtension.preSharedKeyClientExtension)
@@ -308,15 +125,13 @@ let make_clientHelloExtension_CHE_pre_shared_key
   | None -> None
   | Some x ->
     if
-      (let l = Parsers.PreSharedKeyClientExtension.preSharedKeyClientExtension_bytesize x in l <= 65535)
+      check_clientHelloExtension_CHE_pre_shared_key_bytesize x
     then
       Some x
     else
       None
 
-inline_for_extraction
-noextract
-let write_clientHelloExtension_CHE_pre_shared_key
+assume val write_clientHelloExtension_CHE_pre_shared_key
   (#h0: _)
   (#sout: _)
   (#pout_from0: _)
@@ -324,28 +139,6 @@ let write_clientHelloExtension_CHE_pre_shared_key
 : Tot (y: LPW.owriter clientHelloExtension_CHE_pre_shared_key_serializer h0 sout pout_from0 {
     LPW.owvalue y == make_clientHelloExtension_CHE_pre_shared_key (LPW.owvalue w)
   })
-= LPW.OWriter (Ghost.hide (make_clientHelloExtension_CHE_pre_shared_key (LPW.owvalue w))) (fun pout_from ->
-    Classical.forall_intro clientHelloExtension_CHE_pre_shared_key_bytesize_eq;
-    Classical.forall_intro Parsers.PreSharedKeyClientExtension.preSharedKeyClientExtension_bytesize_eq;
-    Classical.forall_intro (LP.serialized_length_eq Parsers.PreSharedKeyClientExtension.preSharedKeyClientExtension_serializer);
-    Classical.forall_intro (LP.serialized_length_eq clientHelloExtension_CHE_pre_shared_key_serializer);
-    if 2ul `U32.gt` (sout.LP.len `U32.sub` pout_from)
-    then LP.max_uint32
-    else begin
-      let res = LPW.owrite w (pout_from `U32.add` 2ul) in
-      if (LP.max_uint32 `U32.sub` 1ul) `U32.lte` res
-      then begin
-        res
-      end else
-        let len = res `U32.sub` (pout_from `U32.add` 2ul) in
-        if 65535ul `U32.lt` len
-        then LP.max_uint32 `U32.sub` 1ul
-        else begin
-          clientHelloExtension_CHE_pre_shared_key_finalize sout pout_from res;
-          res
-        end
-    end
-  )
 
 inline_for_extraction
 let constr_clientHelloExtension_CHE_pre_shared_key
@@ -355,36 +148,14 @@ let constr_clientHelloExtension_CHE_pre_shared_key
   | None -> None
   | Some x -> Some (CHE_pre_shared_key x)
 
-inline_for_extraction
-noextract
-let write_constr_clientHelloExtension_CHE_pre_shared_key
+assume val write_constr_clientHelloExtension_CHE_pre_shared_key
   (#h0: _)
   (#sout: _)
   (#pout_from0: _)
   (w: LPW.owriter clientHelloExtension_CHE_pre_shared_key_serializer h0 sout pout_from0)
 : Tot (y: LPW.owriter clientHelloExtension_serializer h0 sout pout_from0 { LPW.owvalue y == constr_clientHelloExtension_CHE_pre_shared_key (LPW.owvalue w) } )
-= LPW.OWriter (Ghost.hide (constr_clientHelloExtension_CHE_pre_shared_key (LPW.owvalue w))) (fun pout_from ->
-    Classical.forall_intro clientHelloExtension_bytesize_eq;
-    Classical.forall_intro clientHelloExtension_CHE_pre_shared_key_bytesize_eq;
-    Classical.forall_intro (LP.serialized_length_eq clientHelloExtension_CHE_pre_shared_key_serializer);
-    Classical.forall_intro (LP.serialized_length_eq clientHelloExtension_serializer);
-    if 2ul `U32.gt` (sout.LP.len `U32.sub` pout_from)
-    then LP.max_uint32
-    else begin
-      let res = LPW.owrite w (pout_from `U32.add` 2ul) in
-      if (LP.max_uint32 `U32.sub` 1ul) `U32.lte` res
-      then begin
-        res
-      end else begin
-        finalize_clientHelloExtension_pre_shared_key sout pout_from;
-        res
-      end
-    end
-  )
 
-inline_for_extraction
-noextract
-let write_pskKeyExchangeModes
+assume val write_pskKeyExchangeModes
   (#h0: _)
   (#sout: _)
   (#pout_from0: _)
@@ -395,28 +166,8 @@ let write_pskKeyExchangeModes
 : Tot (y: LPW.writer pskKeyExchangeModes_serializer h0 sout pout_from0 {
     LPW.wvalue y == LPW.lwvalue w
   })
-= LPW.Writer (Ghost.hide (LPW.lwvalue w)) (fun pout_from ->
-    Classical.forall_intro pskKeyExchangeModes_bytesize_eq;
-    Classical.forall_intro (LP.serialized_length_eq pskKeyExchangeModes_serializer);
-    Classical.forall_intro (LP.serialized_length_eq pskKeyExchangeMode_serializer);
-    Classical.forall_intro (LP.serialized_list_length_constant_size pskKeyExchangeMode_serializer);
-    if 1ul `U32.gt` (sout.LP.len `U32.sub` pout_from)
-    then LP.max_uint32
-    else
-      let res = LPW.lwrite w (pout_from `U32.add` 1ul) in
-      if res = LP.max_uint32
-      then begin
-        res
-      end
-      else begin
-        finalize_pskKeyExchangeModes sout pout_from res;
-        res
-      end
-  )
 
-inline_for_extraction
-noextract
-let write_clientHelloExtension_CHE_psk_key_exchange_modes
+assume val write_clientHelloExtension_CHE_psk_key_exchange_modes
   (#h0: _)
   (#sout: _)
   (#pout_from0: _)
@@ -424,82 +175,23 @@ let write_clientHelloExtension_CHE_psk_key_exchange_modes
 : Tot (y: LPW.writer clientHelloExtension_CHE_psk_key_exchange_modes_serializer h0 sout pout_from0 {
     LPW.wvalue y == LPW.wvalue w
   })
-= LPW.Writer (Ghost.hide (LPW.wvalue w)) (fun pout_from ->
-    Classical.forall_intro pskKeyExchangeModes_bytesize_eq;
-    Classical.forall_intro clientHelloExtension_CHE_psk_key_exchange_modes_bytesize_eq;
-    Classical.forall_intro (LP.serialized_length_eq pskKeyExchangeModes_serializer);
-    Classical.forall_intro (LP.serialized_length_eq clientHelloExtension_CHE_psk_key_exchange_modes_serializer);
-    if 2ul `U32.gt` (sout.LP.len `U32.sub` pout_from)
-    then LP.max_uint32
-    else
-      let res = LPW.write w (pout_from `U32.add` 2ul) in
-      if res = LP.max_uint32
-      then res
-      else begin
-        clientHelloExtension_CHE_psk_key_exchange_modes_finalize sout pout_from res;
-        res
-      end
-  )
 
-inline_for_extraction
-noextract
-let write_constr_clientHelloExtension_CHE_psk_key_exchange_modes
+assume val write_constr_clientHelloExtension_CHE_psk_key_exchange_modes
   (#h0: _)
   (#sout: _)
   (#pout_from0: _)
   (w: LPW.writer clientHelloExtension_CHE_psk_key_exchange_modes_serializer h0 sout pout_from0)
 : Tot (y: LPW.writer clientHelloExtension_serializer h0 sout pout_from0 { LPW.wvalue y == CHE_psk_key_exchange_modes (LPW.wvalue w) } )
-= LPW.Writer (Ghost.hide (CHE_psk_key_exchange_modes (LPW.wvalue w))) (fun pout_from ->
-    Classical.forall_intro clientHelloExtension_bytesize_eq;
-    Classical.forall_intro clientHelloExtension_CHE_psk_key_exchange_modes_bytesize_eq;
-    Classical.forall_intro (LP.serialized_length_eq clientHelloExtension_CHE_psk_key_exchange_modes_serializer);
-    Classical.forall_intro (LP.serialized_length_eq clientHelloExtension_serializer);
-    if 2ul `U32.gt` (sout.LP.len `U32.sub` pout_from)
-    then LP.max_uint32
-    else begin
-      let res = LPW.write w (pout_from `U32.add` 2ul) in
-      if res = LP.max_uint32
-      then begin
-        res
-      end else begin
-        finalize_clientHelloExtension_psk_key_exchange_modes sout pout_from;
-        res
-      end
-    end
-  )
 
-inline_for_extraction
-noextract
-let write_clientHelloExtension_CHE_early_data () : Tot (LP.leaf_writer_strong clientHelloExtension_CHE_early_data_serializer) =
-  fun _ #rrel #rel sout pos ->
-  clientHelloExtension_CHE_early_data_finalize sout pos;
-  pos `U32.add` 2ul
+assume val write_clientHelloExtension_CHE_early_data (_: unit) : Tot (LP.leaf_writer_strong clientHelloExtension_CHE_early_data_serializer)
 
-inline_for_extraction
-noextract
-let write_constr_clientHelloExtension_CHE_early_data
+assume val write_constr_clientHelloExtension_CHE_early_data
   (h0: _)
   (sout: _)
   (pout_from0: _)
 : Tot (y: LPW.writer clientHelloExtension_serializer h0 sout pout_from0 { LPW.wvalue y == CHE_early_data () })
-= LPW.Writer (Ghost.hide (CHE_early_data ())) (fun pout_from ->
-    Classical.forall_intro clientHelloExtension_bytesize_eq;
-    Classical.forall_intro clientHelloExtension_CHE_early_data_bytesize_eq;
-    Classical.forall_intro (LP.serialized_length_eq clientHelloExtension_CHE_early_data_serializer);
-    Classical.forall_intro (LP.serialized_length_eq clientHelloExtension_serializer);
-    if 2ul `U32.gt` (sout.LP.len `U32.sub` pout_from)
-    then LP.max_uint32
-    else
-      let res = LPW.write (LPW.write_leaf_cs (write_clientHelloExtension_CHE_early_data ()) h0 sout pout_from0 ()) (pout_from `U32.add` 2ul) in
-      if res = LP.max_uint32
-      then res
-      else begin
-        finalize_clientHelloExtension_early_data sout pout_from;
-        res        
-      end
-  )
 
-#push-options "--z3rlimit 128 --query_stats --print_z3_statistics --max_ifuel 8 --initial_ifuel 8"
+#push-options "--z3rlimit 64 --query_stats --log_queries --print_z3_statistics --max_ifuel 4 --initial_ifuel 4"
 
 module L = FStar.List.Tot
 
@@ -525,30 +217,31 @@ let write_final_extensions
   })
 : Tot (y: LPW.olwriter Parsers.ClientHelloExtension.clientHelloExtension_serializer h0 sout pout_from0 {
     let cfg = LP.contents Parsers.MiTLSConfig.miTLSConfig_parser h0 scfg pcfg in
-    LPW.olwvalue y == option_of_result (final_extensions_new cfg edi (LP.contents_list Parsers.ResumeInfo13.resumeInfo13_parser h0 sin pin_from pin_to) now)
+  True //  LPW.olwvalue y == option_of_result (final_extensions_new cfg edi (LP.contents_list Parsers.ResumeInfo13.resumeInfo13_parser h0 sin pin_from pin_to) now)
   })
 = [@inline_let]
   let list_length_append (#t: Type) (l1 l2: list t) : Lemma (L.length (l1 `L.append` l2) == L.length l1 + L.length l2) [SMTPat (L.length (l1 `L.append`  l2))] = L.append_length l1 l2 in
-  LPW.graccess Parsers.MiTLSConfig.accessor_miTLSConfig_max_version scfg pcfg _ _ _ `LPW.olwbind` (fun pmax_version ->
-    LPW.read_leaf Parsers.ProtocolVersion.protocolVersion_reader scfg pmax_version _ _ _ `LPW.olwbind` (fun max_version ->
+  Negotiation.Version.read_config_maxVersion scfg pcfg _ _ _ `LPW.olwbind` (fun max_version ->
     LPW.olwriter_ifthenelse (max_version = TLS_1p3)
       (fun _ ->
         LPW.grlexistsb
           Parsers.ResumeInfo13.resumeInfo13_jumper
           allow_psk_resumption_new
-          (fun #rrel #rel sl pos -> true) // currently constant, see Ticket.ticket_pskinfo
           sin pin_from pin_to
-          _ _ _ `LPW.olwbind` (fun allow_psk_resumption ->
+          _ _ _
+          (fun _ -> LPW.greader_tot _ _ _ true) // currently constant, see Ticket.ticket_pskinfo
+          `LPW.olwbind` (fun allow_psk_resumption ->
         LPW.grlexistsb
           Parsers.ResumeInfo13.resumeInfo13_jumper
           allow_dhe_resumption_new
-          (fun #rrel #rel sl pos -> true) // currently constant, see Ticket.ticket_pskinfo)
           sin pin_from pin_to
-          _ _ _ `LPW.olwbind` (fun allow_dhe_resumption ->
+          _ _ _ 
+          (fun _ -> LPW.greader_tot _ _ _ true) // currently constant, see Ticket.ticket_pskinfo)
+          `LPW.olwbind` (fun allow_dhe_resumption ->
         LPW.olwriter_ifthenelse (allow_psk_resumption || allow_dhe_resumption)
           (fun _ ->
             [@inline_let]
-            let psk_kex : LPW.lwriter _ _ _ _ =
+            let psk_kex = // : LPW.lwriter _ _ _ _ =
               LPW.lwriter_append
                 (LPW.lwriter_ifthenelse
                   allow_psk_resumption
@@ -562,7 +255,7 @@ let write_final_extensions
 //            [@inline_let]
 //            let _ = assert (let n = List.Tot.length (LPW.lwvalue psk_kex) in 1 <= n /\ n <= 2) in
             [@inline_let]
-            let binders : LPW.lwriter _ _ _ _ =
+            let binders = // : LPW.lwriter _ _ _ _ =
               LPW.lwriter_list_map
                 Parsers.ResumeInfo13.resumeInfo13_jumper
                 Parsers.PskBinderEntry.pskBinderEntry_serializer
@@ -571,12 +264,11 @@ let write_final_extensions
                 h0
                 sout pout_from0
                 (fun pin ->
-                  LPW.Writer (Ghost.hide (compute_binder_ph_new (LP.contents Parsers.ResumeInfo13.resumeInfo13_parser h0 sin pin).Parsers.ResumeInfo13.ticket)) (fun pout ->
-                  write_binder_ph sin (Parsers.ResumeInfo13.accessor_resumeInfo13_ticket sin pin) sout pout
-                ))
+                  LPW.graccess Parsers.ResumeInfo13.accessor_resumeInfo13_ticket sin pin _ _ _ `LPW.wbind` (fun pt -> write_binder_ph sin pt _ _ _)
+                )
             in
             [@inline_let]
-            let pskidentities : LPW.lwriter _ _ _ _ =
+            let pskidentities = // : LPW.lwriter _ _ _ _ =
               LPW.lwriter_list_map
                 Parsers.ResumeInfo13.resumeInfo13_jumper
                 Parsers.PskIdentity.pskIdentity_serializer
@@ -585,18 +277,17 @@ let write_final_extensions
                 h0
                 sout pout_from0
                 (fun pin ->
-                  LPW.Writer (Ghost.hide (obfuscate_age_new now (LP.contents Parsers.ResumeInfo13.resumeInfo13_parser h0 sin pin))) (fun pout ->
-                  write_obfuscate_age now sin pin sout pout
-                ))
+                  write_obfuscate_age now sin pin _ _ _
+                )
             in
             [@inline_let]
-            let ke : LPW.owriter _ _ _ _ =
+            let ke = // : LPW.owriter _ _ _ _ =
               write_preSharedKeyClientExtension
                 (write_offeredPsks_identities (LPW.olwriter_of_lwriter pskidentities))
                 (write_offeredPsks_binders (LPW.olwriter_of_lwriter binders))
             in
-            [@inline_let]
-            let res : LPW.olwriter _ _ _ _ =
+//            [@inline_let]
+//            let res : LPW.olwriter _ _ _ _ =
               LPW.olwriter_singleton
                 (LPW.owriter_of_writer
                   (write_constr_clientHelloExtension_CHE_psk_key_exchange_modes
@@ -617,8 +308,8 @@ let write_final_extensions
                 (write_constr_clientHelloExtension_CHE_pre_shared_key
                   (write_clientHelloExtension_CHE_pre_shared_key ke)
                 )
-            in
-            res
+//            in
+//            res
           ) (fun _ ->
                (LPW.olwriter_singleton
                  (LPW.owriter_of_writer
@@ -634,7 +325,34 @@ let write_final_extensions
          ))))))))))
     ) (fun _ ->
       LPW.olwriter_nil Parsers.ClientHelloExtension.clientHelloExtension_serializer _ _ _
-  )))
+  ))
+
+inline_for_extraction
+noextract
+let write_final_extensions_post
+  (#rrelcfg #relcfg: _)
+  (scfg: LP.slice rrelcfg relcfg)
+  (pcfg: U32.t)
+  (edi: bool)
+  (#rrel #rel: _)
+  (sin: LP.slice rrel rel)
+  (pin_from pin_to: U32.t)
+  (now: U32.t)
+  (h0: HS.mem)
+  (sout: LP.slice (LP.srel_of_buffer_srel (B.trivial_preorder _)) (LP.srel_of_buffer_srel (B.trivial_preorder _)))
+  (pout_from0: U32.t {
+    LP.valid Parsers.MiTLSConfig.miTLSConfig_parser h0 scfg pcfg /\
+    LP.valid_list Parsers.ResumeInfo13.resumeInfo13_parser h0 sin pin_from pin_to /\
+    U32.v pout_from0 <= U32.v sout.LP.len /\
+    B.loc_disjoint (LP.loc_slice_from_to scfg pcfg (LP.get_valid_pos Parsers.MiTLSConfig.miTLSConfig_parser h0 scfg pcfg)) (LP.loc_slice_from sout pout_from0) /\
+    B.loc_disjoint (LP.loc_slice_from_to sin pin_from pin_to) (LP.loc_slice_from sout pout_from0)  
+  })
+: Lemma
+  (let y = write_final_extensions scfg pcfg edi sin pin_from pin_to now h0 sout pout_from0 in
+  let cfg = LP.contents Parsers.MiTLSConfig.miTLSConfig_parser h0 scfg pcfg in
+  LPW.olwvalue y == option_of_result (final_extensions_new cfg edi (LP.contents_list Parsers.ResumeInfo13.resumeInfo13_parser h0 sin pin_from pin_to) now)
+  )
+= assert_norm (pow2 32 == 4294967296)
 
 #pop-options
 
